StrataTest/Languages/Boole/loop_simple.lean
@@ -29,19 +29,19 @@ spec {
 };
 #end
 
-/-- info: Obligation: entry_invariant_0_0
+/-- info: Obligation: loopElimAssert_loop_0_entry_invariant_0
 Property: assert
 Result: ✅ pass
 
-Obligation: entry_invariant_0_1
+Obligation: loopElimAssert_loop_0_entry_invariant_1
 Property: assert
 Result: ✅ pass
 
-Obligation: arbitrary_iter_maintain_invariant_0_0
+Obligation: loopElimAssert_loop_0_arbitrary_iter_maintain_invariant_0
 Property: assert
 Result: ✅ pass
 
-Obligation: arbitrary_iter_maintain_invariant_0_1
+Obligation: loopElimAssert_loop_0_arbitrary_iter_maintain_invariant_1
 Property: assert
 Result: ✅ pass
 
